start typing

Superposition_Calculus/First_Order_Type_System.thy
@@ -2,6 +2,96 @@ theory First_Order_Type_System
   imports Nonground_Clause Fun_Extra
 begin
 
+locale typing =
+  fixes is_typed is_welltyped
+  assumes is_typed_if_is_welltyped: "\<And>\<T> expr. is_welltyped \<T> expr \<Longrightarrow> is_typed \<T> expr"
+
+locale explicit_typing =
+  fixes typed welltyped
+  assumes 
+    typed_right_unique: "\<And>\<T>. right_unique (typed \<T>)" and
+    welltyped_right_unique: "\<And>\<T>. right_unique (welltyped \<T>)" and
+    typed_if_welltyped: "\<And>\<T> expr \<tau>. welltyped \<T> expr \<tau> \<Longrightarrow> typed \<T> expr \<tau>"
+begin
+
+definition is_typed where
+  "is_typed \<T> expr \<equiv> \<exists>\<tau>. typed \<T> expr \<tau>"
+
+definition is_welltyped where
+  "is_welltyped \<T> expr \<equiv> \<exists>\<tau>. welltyped \<T> expr \<tau>"
+
+sublocale typing where is_typed = is_typed and is_welltyped = is_welltyped
+   using typed_if_welltyped
+   by unfold_locales (auto simp: is_typed_def is_welltyped_def)
+
+end
+
+locale typing_lifting =
+  sub: typing where is_typed = is_typed_sub and is_welltyped = is_welltyped_sub
+for is_typed_sub is_welltyped_sub :: "'\<T> \<Rightarrow> 'sub \<Rightarrow> bool" +
+fixes 
+  to_set :: "'expr \<Rightarrow> 'sub set"
+begin
+
+definition is_typed where
+  "is_typed \<T> expr \<equiv> \<forall>sub \<in> to_set expr. is_typed_sub \<T> sub"
+
+definition is_welltyped where
+  "is_welltyped \<T> expr \<equiv> \<forall>sub \<in> to_set expr. is_welltyped_sub \<T> sub"
+
+sublocale typing where is_typed = is_typed and is_welltyped = is_welltyped
+proof unfold_locales
+  fix \<T> expr
+  assume "is_welltyped \<T> expr"
+  then show "is_typed \<T> expr"
+    unfolding is_typed_def is_welltyped_def
+    using sub.is_typed_if_is_welltyped
+    by blast
+qed
+
+end
+
+locale context_compatible_typing = explicit_typing +
+  fixes Fun
+  assumes 
+    welltyped_context_compatible: 
+    "\<And>\<T> t t' c \<tau> \<tau>'.
+      welltyped \<T> t \<tau>' \<Longrightarrow>
+      welltyped \<T> t' \<tau>' \<Longrightarrow>
+      welltyped \<T> (Fun\<langle>c; t\<rangle>) \<tau> \<Longrightarrow>
+      welltyped \<T> (Fun\<langle>c; t'\<rangle>) \<tau>" and
+    typed_context_compatible: 
+    "\<And>\<T> t t' c \<tau> \<tau>'.
+      typed \<T> t \<tau>' \<Longrightarrow>
+      typed \<T> t' \<tau>' \<Longrightarrow>
+      typed \<T> (Fun\<langle>c; t\<rangle>) \<tau> \<Longrightarrow>
+      typed \<T> (Fun\<langle>c; t'\<rangle>) \<tau>"
+
+locale clause_typing_lifting =
+  "term": explicit_typing term_typed term_welltyped
+  for term_typed term_welltyped
+begin
+
+sublocale atom: typing_lifting where 
+  is_typed_sub = term.is_typed and 
+  is_welltyped_sub = term.is_welltyped and
+  to_set = set_uprod 
+  by unfold_locales
+
+sublocale literal: typing_lifting where 
+  is_typed_sub = atom.is_typed and 
+  is_welltyped_sub = atom.is_welltyped and
+  to_set = "\<lambda>l. {atm_of l}"
+  by unfold_locales
+
+sublocale clause: typing_lifting where 
+  is_typed_sub = literal.is_typed and 
+  is_welltyped_sub = literal.is_welltyped and
+  to_set = set_mset
+  by unfold_locales
+
+end
+
 type_synonym ('f, 'ty) fun_types = "'f \<Rightarrow> 'ty list \<times> 'ty"
 type_synonym ('v, 'ty) var_types = "'v \<Rightarrow> 'ty"
 
@@ -14,11 +104,6 @@ inductive welltyped :: "('f, 'ty) fun_types \<Rightarrow>  ('v, 'ty) var_types \
   for \<F> \<V> where
     Var: "\<V> x = \<tau> \<Longrightarrow> welltyped \<F> \<V> (Var x) \<tau>"
   | Fun: "\<F> f = (\<tau>s, \<tau>) \<Longrightarrow> list_all2 (welltyped \<F> \<V>) ts \<tau>s \<Longrightarrow> welltyped \<F> \<V> (Fun f ts) \<tau>"
-
-inductive welltyped' :: "('f, 'ty) fun_types \<Rightarrow>  ('v, 'ty) var_types \<Rightarrow> ('f,'v) term \<Rightarrow> 'ty \<Rightarrow> bool" 
-  for \<F> \<V> where
-    Var: "\<V> x = \<tau> \<Longrightarrow> welltyped' \<F> \<V> (Var x) \<tau>"
-  | Fun: "\<F> f = (\<tau>s, \<tau>) \<Longrightarrow> list_all2 (welltyped \<F> \<V>) ts \<tau>s \<Longrightarrow> welltyped' \<F> \<V> (Fun f ts) \<tau>"
 
 lemma has_type_right_unique: "right_unique (has_type \<F> \<V>)"
 proof (rule right_uniqueI)
@@ -34,6 +119,24 @@ proof (rule right_uniqueI)
   assume "welltyped \<F> \<V> t \<tau>\<^sub>1" and "welltyped \<F> \<V> t \<tau>\<^sub>2"
   thus "\<tau>\<^sub>1 = \<tau>\<^sub>2"
     by (auto elim!: welltyped.cases)
+qed
+
+global_interpretation "term": explicit_typing "\<lambda>(\<F>, \<V>). has_type \<F> \<V>" "\<lambda>(\<F>, \<V>). welltyped \<F> \<V>"
+proof(unfold_locales)
+  show "\<And>\<T>. right_unique (case \<T> of (\<F>, \<V>) \<Rightarrow> has_type \<F> \<V>)"
+    using has_type_right_unique
+    by auto
+next
+  show "\<And>\<T>. right_unique (case \<T> of (\<F>, \<V>) \<Rightarrow> welltyped \<F> \<V>)"
+    using welltyped_right_unique
+    by auto
+next
+  fix \<T> and t :: "('f, 'v) term" and \<tau> :: 'ty
+  show "(case \<T> of (\<F>, \<V>) \<Rightarrow> welltyped \<F> \<V>) t \<tau> \<Longrightarrow> (case \<T> of (\<F>, \<V>) \<Rightarrow> has_type \<F> \<V>) t \<tau>"
+    apply(induction t)
+     apply(auto split: prod.splits)
+     apply (simp add: has_type.simps welltyped.simps)
+    using has_type.simps welltyped.cases by fastforce
 qed
 
 definition has_type\<^sub>a where
